src/main.ml
@@ -1,0 +1,34 @@
+open Verified
+
+exception EXIT
+
+let usage () = Format.printf "Usage: vydra MDL LOG\n"; raise EXIT
+
+external init: string -> int = "caml_init"
+external run: int -> (int * string * string list) option = "caml_run"
+external close: unit -> unit = "caml_close"
+
+let _ =
+    let args = List.tl (Array.to_list Sys.argv) in
+    let _ = if List.length args <> 2 then usage () else () in
+    let f =
+        (let ch = open_in (List.nth args 0) in
+        let f = Mdl_parser.formula Mdl_lexer.token (Lexing.from_channel ch) in
+        (close_in ch; f)) in
+    let init_hd = init (List.nth args 1) in
+    let enat_of_ts ts = VYDRA.Enat (VYDRA.nat_of_integer (Z.of_string ts)) in
+    let run_hd e = match run e with
+      | None -> None
+      | Some (e', ts, es) -> Some (e', (enat_of_ts ts, VYDRA.mk_db es)) in
+    let output_nat out t = Z.output out (VYDRA.integer_of_nat t) in
+    let rec fly vydra (ts, tp) = match VYDRA.run_vydra_string_enat run_hd vydra with
+      | None -> close ()
+      | Some (vydra', (et, b)) ->
+        let t = match et with
+          | VYDRA.Enat t -> t in
+        let tp' = match ts with
+          | None -> tp
+          | Some ts' -> if t = ts' then Z.succ tp else Z.zero in
+        let _ = Printf.printf "%a:%a %B\n" output_nat t Z.output tp' b in
+        fly vydra' (Some t, tp') in
+    fly (VYDRA.init_vydra_string_enat init_hd run_hd f) (None, Z.zero)
