src/mdl_parser.mly
@@ -1,0 +1,73 @@
+%{
+open Verified
+let inf_in = VYDRA.interval_enat (VYDRA.Enat (VYDRA.nat_of_integer (Z.of_int 0))) VYDRA.Infinity_enat
+%}
+
+%token <string> ATOM
+%token <Verified.VYDRA.enat Verified.VYDRA.i> INTERVAL
+%token LOPEN ROPEN FORWARD BACKWARD
+%token FALSE TRUE NEG CONJ DISJ PLUS EOF
+%token WILDCARD QUESTION STAR
+%token SINCE UNTIL
+%token PREV NEXT ONCE EVENTUALLY HISTORICALLY ALWAYS
+
+%nonassoc FALSE TRUE WILDCARD
+%nonassoc BACKWARD FORWARD
+%nonassoc PREV NEXT ONCE EVENTUALLY HISTORICALLY ALWAYS
+%left SINCE UNTIL
+%left DISJ
+%left CONJ
+%left PLUS
+%left CONCAT
+%nonassoc NEG
+%nonassoc STAR
+%nonassoc LOPEN
+%nonassoc QUESTION
+%nonassoc INTERVAL
+%nonassoc ATOM
+
+%type <(string, Verified.VYDRA.enat) Verified.VYDRA.formula> formula
+%start formula
+
+%%
+
+formula:
+| f=f EOF { f }
+
+f:
+| LOPEN f=f ROPEN                       { f }
+| FALSE                                 { Verified.VYDRA.Bool false }
+| TRUE                                  { Verified.VYDRA.Bool true }
+| a=ATOM                                { Verified.VYDRA.Atom a }
+| a=ATOM LOPEN ROPEN                    { Verified.VYDRA.Atom a }
+| NEG f=f                               { Verified.VYDRA.Neg f }
+| f=f CONJ g=f                          { Verified.VYDRA.Bin ((fun x y -> x && y), f, g) }
+| f=f DISJ g=f                          { Verified.VYDRA.Bin ((fun x y -> x || y), f, g) }
+| PREV i=INTERVAL f=f                   { Verified.VYDRA.Prev (i, f) }
+| PREV            f=f                   { Verified.VYDRA.Prev (inf_in, f) }
+| NEXT i=INTERVAL f=f                   { Verified.VYDRA.Next (i, f) }
+| NEXT            f=f                   { Verified.VYDRA.Next (inf_in, f) }
+| f=f SINCE i=INTERVAL g=f              { Verified.VYDRA.Since (f, i, g) }
+| f=f SINCE            g=f              { Verified.VYDRA.Since (f, inf_in, g) }
+| f=f UNTIL i=INTERVAL g=f              { Verified.VYDRA.Until (f, i, g) }
+| f=f UNTIL            g=f              { Verified.VYDRA.Until (f, inf_in, g) }
+| ONCE i=INTERVAL f=f                   { Verified.VYDRA.Since (Verified.VYDRA.Bool true, i, f) }
+| ONCE            f=f                   { Verified.VYDRA.Since (Verified.VYDRA.Bool true, inf_in, f) }
+| EVENTUALLY i=INTERVAL f=f             { Verified.VYDRA.Until (Verified.VYDRA.Bool true, i, f) }
+| EVENTUALLY            f=f             { Verified.VYDRA.Until (Verified.VYDRA.Bool true, inf_in, f) }
+| HISTORICALLY i=INTERVAL f=f           { Verified.VYDRA.Neg (Verified.VYDRA.Since (Verified.VYDRA.Bool true, i, Verified.VYDRA.Neg f)) }
+| HISTORICALLY            f=f           { Verified.VYDRA.Neg (Verified.VYDRA.Since (Verified.VYDRA.Bool true, inf_in, Verified.VYDRA.Neg f)) }
+| ALWAYS i=INTERVAL f=f                 { Verified.VYDRA.Neg (Verified.VYDRA.Until (Verified.VYDRA.Bool true, i, Verified.VYDRA.Neg f)) }
+| ALWAYS            f=f                 { Verified.VYDRA.Neg (Verified.VYDRA.Until (Verified.VYDRA.Bool true, inf_in, Verified.VYDRA.Neg f)) }
+| BACKWARD i=INTERVAL r=re              { Verified.VYDRA.MatchP (i, r) } %prec BACKWARD
+| BACKWARD            r=re              { Verified.VYDRA.MatchP (inf_in, r) } %prec BACKWARD
+| FORWARD i=INTERVAL r=re               { Verified.VYDRA.MatchF (i, r) } %prec FORWARD
+| FORWARD            r=re               { Verified.VYDRA.MatchF (inf_in, r) } %prec FORWARD
+
+re:
+| LOPEN r=re ROPEN     { r }
+| WILDCARD             { Verified.VYDRA.Wild }
+| f=f QUESTION         { Verified.VYDRA.Test f }
+| r=re PLUS s=re       { Verified.VYDRA.Plus (r, s) }
+| r=re      s=re       { Verified.VYDRA.Times (r, s) } %prec CONCAT
+| r=re STAR            { Verified.VYDRA.Star r }
