README.md
@@ -1,10 +1,10 @@
-HYDRA is a monitor for metric temporal logic (MTL)
-and metric dynamic logic (MDL).
-The two versions, called HYDRA(MTL) and HYDRA(MDL), respectively,
-are presented in the papers
+# HYDRA
+
+HYDRA is a monitor for metric temporal logic (MTL) and metric dynamic logic (MDL).
+The two versions, called HYDRA(MTL) and HYDRA(MDL), are presented in the papers
 
 Multi-Head Monitoring of Metric Temporal Logic,  
-Multi-Head Monitoring of Metric Dynamic Logic
+Multi-Head Monitoring of Metric Dynamic Logic,
 
 accepted at [ATVA 2019](https://doi.org/10.1007/978-3-030-31784-3_9)
 and [ATVA 2020](https://doi.org/10.1007/978-3-030-59152-6_13), respectively.
@@ -12,7 +12,7 @@ and [ATVA 2020](https://doi.org/10.1007/978-3-030-59152-6_13), respectively.
 This artifact is the supplementary material for these papers.
 
 HYDRA takes as input an MTL or MDL formula and a trace stored in a file
-and outputs a trace of verdicts denoting the satisfaction (or violation)
+and outputs a sequence of verdicts denoting the satisfaction (or violation)
 of the formula at every position in the trace (for formulas involving
 future operators, the trace of verdicts may be incomplete if no verdict
 for a time-point can be inferred by the monitor from the given trace).
@@ -24,14 +24,16 @@ for a time-point can be inferred by the monitor from the given trace).
 - `atva19.pdf` - paper on HYDRA(MTL)
 - `atva20.pdf` - paper on HYDRA(MDL)
 - `Dockerfile` - Dockerfile for this supplementary material
+- `hydra` - HYDRA's executable
+- `vydra` - VYDRA's executable
 - `run_exp.sh` - script to run the experiments (see below for more details)
 - `run_tests.sh` - script to run the correctness tests (see below for more details)
 - `evaluation/` contains tools for running the experiments and correctness tests
-- `examples/` contains example formulas and log from this README
+- `examples/` contains example formulas and logs
 - `html/` contains the generated HTML page of the formalization in Isabelle/HOL
-- `src/` contains HYDRA's source code (in C++)
-- `thys/` contains the formalization of the paper in Isabelle
-- `vydra/` contains the formally verified core (`verified.ml`) and unverified code to parse the formula and trace
+- `src/` contains HYDRA's source code (in C++) and VYDRA's source code (the formally verified core in `verified.ml` and unverified code to parse the formula and trace in OCaml and C)
+- `thys/` contains the formalization of HYDRA(MDL) in Isabelle
+- `aerial/`, `monpoly/`, `pcre2/`, `reelay-codegen/` contain third-party tools for the empirical evaluation
 
 ---
 
@@ -85,13 +87,17 @@ obtain a shell with all the tools installed.
 
 To run HYDRA type:
 ```
-$ ./hydra formula log
+$ ./hydra ${formula} ${log}
+```
+To run VYDRA type:
+```
+$ ./vydra ${formula} ${log}
 ```
 where 
-
-formula = path to a text file with an MTL/MDL formula  
-log     = path to a text file with a log
-
+```
+${formula} = path to a text file with an MTL/MDL formula
+${log}     = path to a text file with a log
+```
 
 MDL Syntax
 
@@ -124,8 +130,8 @@ Non-terminals are enclosed in curly braces.
 
 The semantics of temporal match operators is defined as follows:
 ```
-i |= ◁ [a, b] {r} iff \exists j <= i. \tau_i \in \tau_j + [a, b] /\ (j, i) \in R(r)
-i |= ▷ [a, b] {r} iff \exists j >= i. \tau_j \in \tau_i + [a, b] /\ (i, j) \in R(r)
+i |= ◁ [a, b] {r} iff \exists j <= i. \tau_i - \tau_j \in [a, b] /\ (j, i) \in R(r)
+i |= ▷ [a, b] {r} iff \exists j >= i. \tau_j - \tau_i \in [a, b] /\ (i, j) \in R(r)
 ```
 
 Log Syntax
@@ -151,10 +157,11 @@ p0 OR (▷ [2,2] (p1? .)* p2?)
 $ cat examples/ex.log
 @0 p1 p2
 @0 p0 p2
-@1
-@4 p0 p1 p2
+@1 p1
+@4 p0 p2
 @4 p1 p2
-@5 p0 p1 p2
+@6 p0 p1 p2
+@7 p1
 
 $ ./hydra ./examples/ex.mtl ./examples/ex.log
 Monitoring (p0 OR (p1 UNTIL[2,2] p2))
@@ -162,8 +169,7 @@ Monitoring (p0 OR (p1 UNTIL[2,2] p2))
 0:1 true
 1:0 false
 4:0 true
-4:1 false
-5:0 true
+4:1 true
 Bye.
 
 $ ./hydra ./examples/ex.mdl ./examples/ex.log
@@ -171,7 +177,16 @@ Monitoring (p0 OR (▷ [2,2] ((((p1?) .)*) (p2?))))
 0:0 false
 0:1 true
 1:0 false
+4:0 true
+4:1 true
 Bye.
+
+$ ./vydra ./examples/ex.mdl ./examples/ex.log
+0:0 false
+0:1 true
+1:0 false
+4:0 true
+4:1 true
 ```
 
 ---
@@ -243,4 +258,3 @@ The mapping of the experiment names is summarized here:
 - Experiment WC -> `exp_mtl_exp`
 - Experiment RL -> `exp_mtl_fixed`
 - Experiment RE -> `exp_pcre`
-
